src/proof/kubernetes_model/tx/update_status.v
@@ -105,7 +105,8 @@ Proof.
   iExists uid, (DfracOwn 1), kmeta, None, (Some kstatus).
   iFrame "Hown_meta_frag Hown_status_frag".
   iIntros (existing_i existing_kobj) "Hget".
-  iDestruct "Hget" as "(%Hvalid_existing & %Hkey_existing & %Hmeta_eq &
+  iDestruct "Hget" as "(%Hvalid_existing & %Hextra_valid_existing &
+    %Hkey_existing & %Hmeta_eq &
     Hdeepown_existing_i & Hown_meta_frag & _ & (Hown_status_frag & %Hstatus_eq))".
   iMod ("Habort" with "[Hown_meta_frag Hown_status_frag]") as "Hau".
   { iFrame. iFrame "%". }
